Term subst preserves subcapt, subtype and typing

CC/Subst.lean
@@ -1,24 +1,75 @@
 import Mathlib.Data.Fin.Basic
 import CC.Basic
+import CC.CaptureSet
 import CC.Type
+import CC.Type.TypeSubst
 import CC.Context
+import CC.TypeMap
+import CC.Typed
+import CC.Subtype
+import CC.Term
+import CC.Typed.Rename
 
 namespace CC
 
-def OpenMap (n m : Nat) : Type :=
-  Fin m.succ -> PType n m
+def VarSubst (Γ : Ctx n1 m) (Δ : Ctx n2 m) (f : VarMap n1 n2) : Prop :=
+  ∀ {x T}, BoundVar Γ x T -> Typed Δ (Term.var (f x)) {f x} (T.rename f id)
 
-def OpenMap.ext_var (σ : OpenMap n m) : OpenMap n.succ m :=
-  fun x => (σ x).weaken_var
+def TVarSubst (Γ : Ctx n m1) (Δ : Ctx n m2) (g : TypeMap n m1 m2) : Prop :=
+  ∀ {X S}, BoundTVar Γ X S -> SubtypeP Δ (g X) (S.tsubst g)
 
-def OpenMap.ext_tvar (σ : OpenMap n m) : OpenMap n m.succ := by
-  intro x
-  cases x using Fin.cases with
-  | H0 => exact PType.tvar 0
-  | Hs x0 => exact (σ x0).weaken_tvar
+theorem Typed.var_bound_type :
+  BoundVar Γ x T ->
+  Typed Γ (Term.var x) {x} T := by
+  intro hb
+  cases T
+  apply Typed.sub
+  apply Typed.var
+  trivial
+  apply Subtype.capt
+  apply Subcapt.sc_var
+  exact hb
+  constructor
 
-def tvar_open_map (R : PType n m) : OpenMap n m := by
-  intro x
-  cases x using Fin.cases with
-  | H0 => exact R
-  | Hs x0 => exact PType.tvar x0
+def VarSubst.ext_var (σ : VarSubst Γ Δ f) P :
+  VarSubst (Ctx.extend_var Γ P) (Ctx.extend_var Δ (P.rename f id)) f.ext := by
+  intros x T h
+  cases h
+  case here =>
+    conv =>
+      arg 2
+      simp [VarMap.ext]
+    conv =>
+      arg 3
+      simp [VarMap.ext]
+    rw [<- CType.rename_weaken_comm]
+    apply Typed.var_bound_type
+    constructor
+  case there_var h =>
+    conv =>
+      arg 2
+      simp [VarMap.ext]
+    conv =>
+      arg 3
+      simp [VarMap.ext]
+    rw [<- CType.rename_weaken_comm]
+    have h' := σ h
+    have h'' := h'.weaken_var (P.rename f id)
+    exact h''
+
+def VarSubst.ext_tvar (σ : VarSubst Γ Δ f) R :
+  VarSubst (Ctx.extend_tvar Γ R) (Ctx.extend_tvar Δ (R.rename f id)) f := by
+  intros X T h
+  cases h
+  case there_tvar h =>
+    conv =>
+      arg 2
+      simp [VarMap.ext]
+    conv =>
+      arg 3
+      simp [VarMap.ext]
+    rw [<- id_ext]
+    rw [<- CType.rename_weaken_tvar_comm]
+    have h' := σ h
+    have h'' := h'.weaken_tvar (R.rename f id)
+    exact h''
