CC/Typed.lean
@@ -3,20 +3,31 @@ import CC.CaptureSet
 import CC.Basic
 import CC.CaptureSet
 import CC.Type
-import CC.Type.Subst
+import CC.Type.TypeSubst
 import CC.Term
 import CC.Context
 import CC.Subtype
 
 namespace CC
 
+inductive DropBinderFree : CaptureSet n.succ -> CaptureSet n -> Prop where
+  | drop : DropBinderFree C.weaken_var C
+
+inductive DropBinder : CaptureSet n.succ -> CaptureSet n -> Prop where
+  | drop_free : DropBinderFree C C' -> DropBinder C C'
+  | drop : DropBinder (C.weaken_var ∪ {0}) C
+
 inductive Typed : Ctx n m -> Term n m -> CaptureSet n -> CType n m -> Prop where
 | var :
-  BoundVar Γ x T ->
-  Typed Γ (Term.var x) {x} T
+  BoundVar Γ x (CType.capt C S) ->
+  Typed Γ (Term.var x) {x} (CType.capt {x} S)
+| sub :
+  Typed Γ t C T ->
+  Subtype Γ T T' ->
+  Typed Γ t C T'
 | abs :
   Typed (Ctx.extend_var Γ T) t C U ->
-  C = C'.weaken_var ∨ C = C'.weaken_var ∪ {0} ->
+  DropBinder C C' ->
   Typed Γ (Term.abs T t) C' (CType.capt C' (PType.arr T U))
 | tabs :
   Typed (Ctx.extend_tvar Γ S) t C T ->
@@ -38,12 +49,12 @@ inductive Typed : Ctx n m -> Term n m -> CaptureSet n -> CType n m -> Prop where
   Typed Γ t Ct T ->
   Typed (Ctx.extend_var Γ T) u Cu U ->
   U = U'.weaken_var ->
-  Cu = Cu'.weaken_var ∨ Cu = Cu'.weaken_var ∪ {0} ->
+  DropBinder Cu Cu' ->
   Typed Γ (Term.letval t u) (Ct ∪ Cu') U'
 | letval2 : ∀ {Γ : Ctx n m} {U' : CType n m} {Cu' : CaptureSet n},
   Typed Γ v Ct T ->
   Value v ->
   Typed (Ctx.extend_var Γ T) u Cu U ->
   U = U'.weaken_var ->
-  Cu = Cu'.weaken_var ->
+  DropBinderFree Cu Cu' ->
   Typed Γ (Term.letval v u) Cu' U'
