CC/CaptureSet.lean
@@ -34,6 +34,12 @@ theorem rename_singleton (x : Fin n) (f : VarMap n n') :
   simp [CaptureSet.rename]
   aesop
 
+@[simp]
+theorem rename_empty (f : VarMap n n') :
+  CaptureSet.rename ∅ f = ∅ := by
+  simp [CaptureSet.rename]
+  aesop
+
 theorem mem_def {x : Fin n} {C : CaptureSet n} : x ∈ C ↔ x ∈ C.1 := Iff.rfl
 
 theorem mem_rename_of_mem (f : VarMap n1 n2) {C : CaptureSet n1} (h : x ∈ C) : f x ∈ C.rename f := by
@@ -46,6 +52,8 @@ theorem mem_rename {C : CaptureSet n} :
   y ∈ C.rename f ↔ ∃ x ∈ C, f x = y := by
   simp only [CaptureSet.rename, mem_def]
   aesop
+
+theorem union_def {C1 C2 : CaptureSet n} : C1 ∪ C2 = ⟨C1.1 ∪ C2.1⟩ := rfl
 
 @[simp]
 theorem CaptureSet.rename_id : ∀ {C : CaptureSet n},
@@ -63,3 +71,8 @@ theorem CaptureSet.rename_comp {C : CaptureSet n1} {f1 : VarMap n1 n2} {f2 : Var
   (C.rename f1).rename f2 = C.rename (f2.comp f1) := by
   unfold VarMap.comp
   simp [CaptureSet.rename, Finset.image_image]
+
+theorem CaptureSet.rename_union {C1 C2 : CaptureSet n} :
+  (C1 ∪ C2).rename f = C1.rename f ∪ C2.rename f := by
+  simp [CaptureSet.rename, union_def, Finset.image_union]
+  
