CC/Rename.lean
@@ -10,6 +10,40 @@ def VarRename (Γ : Ctx n1 m1) (Δ : Ctx n2 m2) (f : VarMap n1 n2) (g : VarMap m
 def TVarRename (Γ : Ctx n1 m1) (Δ : Ctx n2 m2) (f : VarMap n1 n2) (g : VarMap m1 m2) : Prop :=
   ∀ {X S}, BoundTVar Γ X S -> BoundTVar Δ (g X) (S.rename f g)
 
+def VarRename.weaken_var_map (Γ : Ctx n m) (T : CType n m) :
+  VarRename Γ (Ctx.extend_var Γ T) weaken_map id := by
+  intro x P h
+  apply BoundVar.there_var
+  trivial
+
+def TVarRename.weaken_var_map (Γ : Ctx n m) (T : CType n m) :
+  TVarRename Γ (Ctx.extend_var Γ T) weaken_map id := by
+  intro X P h
+  apply BoundTVar.there_var
+  trivial
+
+def VarRename.weaken_tvar_map (Γ : Ctx n m) (S : PType n m) :
+  VarRename Γ (Ctx.extend_tvar Γ S) id weaken_map := by
+  intro x P h
+  apply BoundVar.there_tvar
+  trivial
+
+def TVarRename.weaken_tvar_map (Γ : Ctx n m) (S : PType n m) :
+  TVarRename Γ (Ctx.extend_tvar Γ S) id weaken_map := by
+  intro X P h
+  apply BoundTVar.there_tvar
+  trivial
+
+theorem CaptureSet.rename_weaken_var_comp (C : CaptureSet n) :
+  C.weaken_var.rename f = C.rename (f.comp weaken_map) := by
+  simp [weaken_var]
+  simp [CaptureSet.rename_comp]
+
+theorem CaptureSet.weaken_var_rename_comp (C : CaptureSet n) :
+  (C.rename f).weaken_var = C.rename (weaken_map.comp f) := by
+  simp [weaken_var]
+  simp [CaptureSet.rename_comp]
+
 theorem CType.rename_weaken_var_comp (T : CType n m) :
   T.weaken_var.rename f g = T.rename (f.comp weaken_map) g := by
   simp [weaken_var]
@@ -19,6 +53,26 @@ theorem CType.rename_weaken_tvar_comp (T : CType n m) :
   T.weaken_tvar.rename f g = T.rename f (g.comp weaken_map) := by
   simp [weaken_tvar]
   simp [CType.rename_comp]
+
+theorem CType.rename_open_comp 
+  {n m : Nat} (T : CType n.succ m) 
+  {x : Fin n} {f : VarMap n n'} {g : VarMap m m'} :
+  (T.open_var x).rename f g = T.rename (f.comp (open_map x)) g := by
+  simp [open_var]
+  simp [CType.rename_comp]
+
+theorem CType.open_rename_comp {n1 n2 m1 m2} (T : CType n1 m1)
+  {x : Fin n2} {f : VarMap n1 n2.succ} {g : VarMap m1 m2} :
+  (T.rename f g).open_var x = T.rename ((open_map x).comp f) g := by
+  simp [open_var]
+  simp [CType.rename_comp]
+
+theorem CType.rename_open_comm {n1 n2 m1 m2} (T : CType n1.succ m1)
+  {x : Fin n1} {f : VarMap n1 n2} {g : VarMap m1 m2} :
+  (T.open_var x).rename f g = (T.rename f.ext g).open_var (f x) := by
+  simp [CType.rename_open_comp]
+  simp [comp_open]
+  rw [<- CType.open_rename_comp]
 
 theorem PType.rename_weaken_var_comp (S : PType n m) :
   S.weaken_var.rename f g = S.rename (f.comp weaken_map) g := by
@@ -49,6 +103,31 @@ theorem PType.weaken_var_rename_comp (S : PType n m) :
   (S.rename f g).weaken_var = S.rename (weaken_map.comp f) g := by
   simp [weaken_var]
   simp [PType.rename_comp]
+
+theorem CType.rename_weaken_comm (T : CType n m) :
+  (T.rename f g).weaken_var = T.weaken_var.rename f.ext g := by
+  simp [CType.rename_weaken_var_comp]
+  rw [<- CType.weaken_var_rename_comp]
+
+theorem PType.rename_weaken_comm (S : PType n m) :
+  (S.rename f g).weaken_var = S.weaken_var.rename f.ext g := by
+  simp [PType.rename_weaken_var_comp]
+  rw [<- PType.weaken_var_rename_comp]
+
+theorem PType.rename_weaken_tvar_comm (S : PType n m) :
+  (S.rename f g).weaken_tvar = S.weaken_tvar.rename f g.ext := by
+  simp [PType.rename_weaken_tvar_comp]
+  rw [<- PType.weaken_tvar_rename_comp]
+
+theorem CType.rename_weaken_tvar_comm (T : CType n m) :
+  (T.rename f g).weaken_tvar = T.weaken_tvar.rename f g.ext := by
+  simp [CType.rename_weaken_tvar_comp]
+  rw [<- CType.weaken_tvar_rename_comp]
+
+theorem CaptureSet.rename_weaken_comm (C : CaptureSet n) :
+  (C.rename f).weaken_var = C.weaken_var.rename f.ext := by
+  simp [CaptureSet.rename_weaken_var_comp]
+  rw [<- CaptureSet.weaken_var_rename_comp]
 
 def VarRename.ext_var {Γ : Ctx n1 m1} {Δ : Ctx n2 m2} 
   (σ : VarRename Γ Δ f g) (T : CType n1 m1) :
@@ -103,3 +182,7 @@ def TVarRename.ext_tvar {Γ : Ctx n1 m1} {Δ : Ctx n2 m2}
     rw [<- PType.weaken_tvar_rename_comp]
     constructor
     aesop
+
+def CType.rename_split (T : CType n m) :
+  T.rename f g = (T.rename id g).rename f id := by
+  simp [CType.rename_comp]
