CC/Subcapt/Basic.lean
@@ -1,0 +1,18 @@
+import Mathlib.Data.Fin.Basic
+import CC.Basic
+import CC.CaptureSet
+import CC.Type
+import CC.Context
+import CC.TypeMap
+import CC.Subst
+import CC.Typed
+import CC.Subcapt
+
+namespace CC
+
+def Subcapt.refl :
+  Subcapt Γ C C := by
+  apply Subcapt.sc_set
+  intro x0 h
+  apply Subcapt.sc_elem
+  aesop
