CC/Subcapt/Subst.lean
@@ -1,0 +1,40 @@
+import Mathlib.Data.Fin.Basic
+import CC.Basic
+import CC.CaptureSet
+import CC.Type
+import CC.Context
+import CC.TypeMap
+import CC.Subst
+import CC.Typed
+import CC.Typed.Basic
+import CC.Subcapt
+
+namespace CC
+
+def Subcapt.subst (σ : VarSubst Γ Δ f) :
+  Subcapt Γ C1 C2 ->
+  Subcapt Δ (C1.rename f) (C2.rename f) := by
+  intro h
+  induction h
+  case sc_trans ih1 ih2 =>
+    apply Subcapt.sc_trans
+    apply ih1; aesop
+    apply ih2; aesop
+  case sc_elem h =>
+    simp
+    apply Subcapt.sc_elem
+    apply mem_rename_of_mem; assumption
+  case sc_var h =>
+    simp
+    have h' := σ h
+    simp [CType.rename] at h'
+    apply Typed.var_inv_subcapt; aesop
+  case sc_set hs =>
+    apply Subcapt.sc_set
+    intro x1 h1
+    rw [mem_rename] at h1
+    let ⟨x2, ⟨h2, eq2⟩⟩ := h1
+    have h := hs x2 h2 σ
+    rw [rename_singleton] at h
+    rw [<- eq2]
+    assumption
