CC/Subtype/Subst.lean
@@ -1,0 +1,76 @@
+import Mathlib.Data.Fin.Basic
+import CC.Basic
+import CC.Rename
+import CC.CaptureSet
+import CC.Type
+import CC.Context
+import CC.TypeMap
+import CC.Subst
+import CC.Typed
+import CC.Typed.Basic
+import CC.Subtype
+import CC.Subcapt.Subst
+
+namespace CC
+
+def SubtypeP.subst (σ : VarSubst Γ Δ f) (δ : TVarRename Γ Δ f id) :
+  SubtypeP Γ T1 T2 ->
+  SubtypeP Δ (T1.rename f id) (T2.rename f id) := by
+  intro h
+  apply SubtypeP.rec
+        (motive_1 := 
+          fun Γ T1 T2 _ => 
+            ∀ {n2} {Δ : Ctx n2 _} {f} {_ : VarSubst Γ Δ f} {_ : TVarRename Γ Δ f id}, Subtype Δ (T1.rename f id) (T2.rename f id))
+        (motive_2 := 
+          fun Γ S1 S2 _ =>
+            ∀ {n2} {Δ : Ctx n2 _} {f} {_ : VarSubst Γ Δ f} {_ : TVarRename Γ Δ f id}, SubtypeP Δ (S1.rename f id) (S2.rename f id))
+    <;> try assumption
+  case capt => 
+    intros
+    simp [CType.rename]
+    apply Subtype.capt
+    apply Subcapt.subst <;> aesop
+    aesop
+  case refl =>
+    intros; constructor
+  case trans =>
+    intros
+    apply SubtypeP.trans <;> aesop
+  case top =>
+    intros; simp [PType.rename]; apply SubtypeP.top
+  case tvar =>
+    intros
+    simp [PType.rename]
+    apply SubtypeP.tvar
+    rename_i hb _ _ _ _ δ
+    have h1 := δ hb
+    exact h1
+  case arr =>
+    intros; rename_i ih1 ih2 _ _ f σ δ
+    simp [PType.rename]
+    apply SubtypeP.arr
+    aesop
+    apply ih2
+    apply VarSubst.ext_var; trivial
+    apply TVarRename.ext_var; trivial
+  case tarr =>
+    intros; rename_i ih1 ih2 _ _ f σ δ
+    simp [PType.rename]
+    apply SubtypeP.tarr
+    aesop
+    apply ih2
+    apply VarSubst.ext_tvar; trivial
+    rw [<- id_ext]
+    apply TVarRename.ext_tvar; trivial
+  case boxed =>
+    intros; rename_i ih _ _ f σ δ
+    simp [PType.rename]
+    apply SubtypeP.boxed
+    aesop
+
+def Subtype.subst (h : Subtype Γ T1 T2) (σ : VarSubst Γ Δ f) (δ : TVarRename Γ Δ f id) :
+  Subtype Δ (T1.rename f id) (T2.rename f id) := by
+  cases h
+  constructor
+  apply Subcapt.subst <;> aesop
+  apply SubtypeP.subst <;> aesop
