CC/Type/TypeSubst.lean
@@ -1,0 +1,96 @@
+import CC.Basic
+import CC.Type
+import CC.Context
+import CC.TypeMap
+
+namespace CC
+
+def PType.tsubst (S : PType n m1) (σ : TypeMap n m1 m2) : PType n m2 :=
+  match S with
+  | PType.tvar X => σ X
+  | PType.top => PType.top
+  | PType.arr (CType.capt C1 S1) (CType.capt C2 S2) =>
+    PType.arr (CType.capt C1 (S1.tsubst σ)) (CType.capt C2 (S2.tsubst σ.ext_var))
+  | PType.tarr S1 (CType.capt C2 S2) =>
+    PType.tarr (S1.tsubst σ) (CType.capt C2 (S2.tsubst σ.ext_tvar))
+  | PType.boxed (CType.capt C1 S1) =>
+    PType.boxed (CType.capt C1 (S1.tsubst σ))
+
+def CType.tsubst (T : CType n m1) (σ : TypeMap n m1 m2) : CType n m2 :=
+  match T with
+  | CType.capt C S => CType.capt C (S.tsubst σ)
+
+def CType.open_tvar (T : CType n m.succ) (R : PType n m) : CType n m :=
+  T.tsubst (tvar_open_map R)
+
+def PType.open_tvar (S : PType n m.succ) (R : PType n m) : PType n m :=
+  S.tsubst (tvar_open_map R)
+
+theorem PType.rename_tsubst (T : PType n1 m1)
+  {σ : TypeMap n1 m1 m2} {f : VarMap n1 n2} {g : VarMap m2 m3} :
+  (T.tsubst σ).rename f g = (T.rename f id).tsubst (σ.then f g) :=
+  match T with
+  | PType.tvar X => by
+    simp [tsubst, rename, TypeMap.then]
+  | PType.top => by
+    simp [tsubst, rename, TypeMap.then]
+  | PType.arr (CType.capt C1 S1) (CType.capt C2 S2) => by
+    have ih1 := PType.rename_tsubst S1 (σ := σ) (f := f) (g := g)
+    have ih2 := PType.rename_tsubst S2 (σ := σ.ext_var) (f := f.ext) (g := g)
+    simp [rename, tsubst, ih1]
+    rw [<- TypeMap.ext_var_then_comm]
+    simp [ih2]
+  | PType.tarr S1 (CType.capt C2 S2) => by
+    have ih1 := PType.rename_tsubst S1 (σ := σ) (f := f) (g := g)
+    have ih2 := PType.rename_tsubst S2 (σ := σ.ext_tvar) (f := f) (g := g.ext)
+    simp [rename, tsubst, ih1]
+    rw [<- TypeMap.ext_tvar_then_comm]
+    simp [ih2]
+  | PType.boxed (CType.capt C1 S1) => by
+    have ih1 := PType.rename_tsubst S1 (σ := σ) (f := f) (g := g)
+    simp [rename, tsubst, ih1]
+
+theorem CType.rename_tsubst (T : CType n1 m1)
+  {σ : TypeMap n1 m1 m2} {f : VarMap n1 n2} {g : VarMap m2 m3} :
+  (T.tsubst σ).rename f g = (T.rename f id).tsubst (σ.then f g) := by
+  cases T
+  simp [rename, tsubst, PType.rename_tsubst]
+
+theorem PType.tsubst_rename (T : PType n1 m1)
+  {f : VarMap n1 n2} {g : VarMap m1 m2} {σ : TypeMap n2 m2 m3} :
+  (T.rename f g).tsubst σ = (T.rename f id).tsubst (σ.compv g) :=
+  match T with
+  | PType.tvar X => by
+    simp [tsubst, rename, TypeMap.compv]
+  | PType.top => by
+    simp [tsubst, rename, TypeMap.compv]
+  | PType.arr (CType.capt C1 S1) (CType.capt C2 S2) => by
+    have ih1 := PType.tsubst_rename S1 (f := f) (g := g) (σ := σ)
+    have ih2 := PType.tsubst_rename S2 (f := f.ext) (g := g) (σ := σ.ext_var)
+    simp [rename, tsubst, ih1]
+    simp [TypeMap.compv_ext_var_comm]
+    aesop
+  | PType.tarr S1 (CType.capt C2 S2) => by
+    have ih1 := PType.tsubst_rename S1 (f := f) (g := g) (σ := σ)
+    have ih2 := PType.tsubst_rename S2 (f := f) (g := g.ext) (σ := σ.ext_tvar)
+    simp [rename, tsubst, ih1]
+    simp [TypeMap.compv_ext_tvar_comm]
+    aesop
+  | PType.boxed (CType.capt C1 S1) => by
+    have ih1 := PType.tsubst_rename S1 (f := f) (g := g) (σ := σ)
+    simp [rename, tsubst, ih1]
+
+theorem CType.tsubst_rename (T : CType n1 m1)
+  {f : VarMap n1 n2} {g : VarMap m1 m2} {σ : TypeMap n2 m2 m3} :
+  (T.rename f g).tsubst σ = (T.rename f id).tsubst (σ.compv g) := by
+  cases T
+  simp [rename, tsubst]
+  rw [PType.tsubst_rename]
+
+theorem CType.rename_open_tvar_comm (T : CType n1 m1.succ)
+  {R : PType n1 m1} {f : VarMap n1 n2} {g : VarMap m1 m2} :
+  (T.open_tvar R).rename f g = (T.rename f g.ext).open_tvar (R.rename f g) := by
+  unfold CType.open_tvar
+  simp [CType.rename_tsubst]
+  rw [tvar_open_map_rename_comm]
+  rw [<- CType.tsubst_rename]
