CC/TypeMap.lean
@@ -1,0 +1,93 @@
+import Mathlib.Data.Fin.Basic
+import CC.Basic
+import CC.Type
+import CC.Context
+import CC.Rename
+
+namespace CC
+
+def TypeMap (n m1 m2 : Nat) : Type :=
+  Fin m1 -> PType n m2
+
+def TypeMap.ext_var (σ : TypeMap n m1 m2) : TypeMap n.succ m1 m2 :=
+  fun x => (σ x).weaken_var
+
+def TypeMap.ext_tvar (σ : TypeMap n m1 m2) : TypeMap n m1.succ m2.succ := by
+  intro x
+  cases x using Fin.cases with
+  | H0 => exact PType.tvar 0
+  | Hs x0 => exact (σ x0).weaken_tvar
+
+def TypeMap.then (σ : TypeMap n1 m1 m2) (f : VarMap n1 n2) (g : VarMap m2 m3) :
+  TypeMap n2 m1 m3 := fun x => (σ x).rename f g
+
+def TypeMap.compv (σ : TypeMap n m2 m3) (g : VarMap m1 m2) :
+  TypeMap n m1 m3 := fun x => σ (g x)
+
+def tvar_open_map (R : PType n m) : TypeMap n m.succ m := by
+  intro x
+  cases x using Fin.cases with
+  | H0 => exact R
+  | Hs x0 => exact PType.tvar x0
+
+theorem TypeMap.ext_var_then_comm (σ : TypeMap n m1 m2) :
+  σ.ext_var.then f.ext g = (σ.then f g).ext_var := by
+  funext x
+  cases m1 with
+  | zero =>
+    exfalso
+    let ⟨ _ , h ⟩ := x
+    cases h
+  | succ _ =>
+    cases x using Fin.cases with
+    | H0 =>
+      simp [TypeMap.then, TypeMap.ext_var]
+      simp [PType.rename_weaken_comm]
+    | Hs x0 =>
+      simp [TypeMap.then, TypeMap.ext_var]
+      simp [PType.rename_weaken_comm]
+
+theorem TypeMap.ext_tvar_then_comm (σ : TypeMap n m1 m2) :
+  σ.ext_tvar.then f g.ext = (σ.then f g).ext_tvar := by
+  funext x
+  cases x using Fin.cases with
+  | H0 =>
+    simp [TypeMap.then, TypeMap.ext_tvar]
+    simp [PType.rename_weaken_comm, PType.rename]
+  | Hs x0 =>
+    simp [TypeMap.then, TypeMap.ext_tvar]
+    simp [PType.rename_weaken_tvar_comm, PType.rename]
+
+theorem TypeMap.compv_ext_var_comm (σ : TypeMap n m1 m2) :
+  (σ.compv g).ext_var = σ.ext_var.comp g := by aesop
+
+theorem TypeMap.compv_ext_tvar_comm (σ : TypeMap n m1 m2) :
+  (σ.compv g).ext_tvar = σ.ext_tvar.comp g.ext := by
+  funext x
+  cases x using Fin.cases with
+  | H0 => 
+    simp [VarMap.ext]
+    simp [ext_tvar]
+  | Hs x0 =>
+    simp [VarMap.ext]
+    simp [ext_tvar, compv]
+
+theorem tvar_open_map_rename_comm 
+  (R : PType n1 m1)
+  {f : VarMap n1 n2} {g : VarMap m1 m2} :
+  (tvar_open_map R).then f g = (tvar_open_map (R.rename f g)).compv g.ext := by
+  funext x
+  cases x using Fin.cases with
+  | H0 => 
+    conv =>
+      lhs
+      simp [TypeMap.then, tvar_open_map]
+  | Hs x0 =>
+    conv =>
+      lhs
+      simp [TypeMap.then, tvar_open_map]
+    conv =>
+      rhs
+      simp [TypeMap.compv, VarMap.ext]
+      simp [tvar_open_map]
+    simp [PType.rename]
