CC/Typed/Basic.lean
@@ -1,0 +1,40 @@
+import Mathlib.Data.Fin.Basic
+import CC.Basic
+import CC.CaptureSet
+import CC.Type
+import CC.Context
+import CC.TypeMap
+import CC.Typed
+import CC.Subcapt
+import CC.Subcapt.Basic
+
+namespace CC
+
+theorem Typed.var_inv_subcapt' : 
+  t0 = Term.var x ->
+  T0 = CType.capt C S ->
+  Typed Γ t0 Cx T0 ->
+  Subcapt Γ {x} C := by
+  intro eq1 eq2 h
+  induction h 
+  case var =>
+    cases eq1
+    cases eq2
+    apply Subcapt.refl
+  case sub ih =>
+    rename_i T T' _ _
+    cases T
+    have ih := ih eq1 rfl
+    rename_i hsub _
+    cases hsub
+    rename_i hsub _
+    cases eq2
+    apply Subcapt.sc_trans
+    exact ih
+    aesop
+  all_goals cases eq1
+
+theorem Typed.var_inv_subcapt :
+  Typed Γ (Term.var x) Cx (CType.capt C S) ->
+  Subcapt Γ {x} C := by
+  apply Typed.var_inv_subcapt' <;> aesop
