CC/Typed/Rename.lean
@@ -1,0 +1,137 @@
+import Mathlib.Data.Finset.Basic
+import Mathlib.Data.Finset.Image
+
+import CC.Basic
+import CC.Rename
+
+import CC.CaptureSet
+import CC.Context
+import CC.Term
+import CC.Type
+import CC.Subtype
+import CC.Subtype.Rename
+import CC.Typed
+
+namespace CC
+
+def DropBinderFree.rename (h : DropBinderFree C C') :
+  DropBinderFree (C.rename f.ext) (C'.rename f) := by
+  cases h
+  rw [<- CaptureSet.rename_weaken_comm]
+  constructor
+
+def DropBinder.rename (h : DropBinder C C') :
+  DropBinder (C.rename f.ext) (C'.rename f) := by
+  cases h
+  case drop_free =>
+    apply DropBinder.drop_free
+    apply DropBinderFree.rename
+    assumption
+  case drop =>
+    simp [CaptureSet.rename_union]
+    rw [<- CaptureSet.rename_weaken_comm]
+    apply DropBinder.drop
+
+def Typed.rename {Γ : Ctx n1 m1} (h : Typed Γ t C T)
+  {Δ : Ctx n2 m2}
+  (σ : VarRename Γ Δ f g)
+  (δ : TVarRename Γ Δ f g) :
+  Typed Δ (t.rename f g) (C.rename f) (T.rename f g) := by
+  induction h generalizing n2 m2 Δ
+  case var =>
+    simp [Term.rename]
+    apply Typed.var
+    rename_i hb
+    have hb' := σ hb
+    simp [CType.rename] at hb'
+    exact hb'
+  case sub =>
+    apply Typed.sub
+    aesop
+    apply Subtype.rename <;> aesop
+  case abs =>
+    simp [Term.rename]
+    apply Typed.abs
+    rename_i ih
+    apply ih
+    apply σ.ext_var
+    apply δ.ext_var
+    apply DropBinder.rename
+    assumption
+  case tabs =>
+    simp [Term.rename]
+    apply Typed.tabs
+    rename_i ih
+    apply ih
+    apply σ.ext_tvar
+    apply δ.ext_tvar
+  case app =>
+    simp [Term.rename]
+    simp [CType.rename_open_comm, CaptureSet.rename_union]
+    rename_i ih1 ih2
+    have ih1' := ih1 σ δ
+    have ih2' := ih2 σ δ
+    simp [Term.rename] at ih1' ih2'
+    apply Typed.app
+    apply ih1'
+    apply ih2'
+  case tapp => 
+    simp [Term.rename]
+    simp [CType.rename_open_tvar_comm]
+    rename_i ih
+    have ih' := ih σ δ
+    apply Typed.tapp
+    simp [Term.rename] at ih'
+    apply ih'
+  case box =>
+    simp [Term.rename]
+    apply Typed.box
+    rename_i ih
+    apply ih <;> aesop
+  case unbox =>
+    simp [Term.rename]
+    simp [CaptureSet.rename_union]
+    apply Typed.unbox
+    rename_i ih
+    have ih' := ih σ δ
+    simp [Term.rename] at ih'
+    apply ih'
+  case letval1 => 
+    simp [Term.rename]
+    simp [CaptureSet.rename_union]
+    rename_i ih1 ih2
+    apply Typed.letval1
+    apply ih1 <;> aesop
+    apply ih2
+    apply VarRename.ext_var; trivial
+    apply TVarRename.ext_var; trivial
+    subst_vars
+    simp [CType.rename_weaken_comm]
+    apply DropBinder.rename; trivial
+  case letval2 ih1 ih2 => 
+    simp [Term.rename]
+    apply Typed.letval2
+    apply ih1 <;> trivial
+    apply Value.rename; trivial
+    apply ih2
+    apply VarRename.ext_var; trivial
+    apply TVarRename.ext_var; trivial
+    subst_vars
+    simp [CType.rename_weaken_comm]
+    apply DropBinderFree.rename; trivial
+
+def Typed.weaken_var (h : Typed Γ t C T) P :
+   Typed (Ctx.extend_var Γ P) t.weaken_var C.weaken_var T.weaken_var := by
+   apply Typed.rename
+   exact h
+   apply VarRename.weaken_var_map
+   apply TVarRename.weaken_var_map
+
+def Typed.weaken_tvar (h : Typed Γ t C T) P :
+   Typed (Ctx.extend_tvar Γ P) t.weaken_tvar C T.weaken_tvar := by
+   have heq : C.rename id = C := by simp [CaptureSet.rename]
+   rw [<- heq]
+   apply Typed.rename
+   exact h
+   apply VarRename.weaken_tvar_map
+   apply TVarRename.weaken_tvar_map
