CC/Typed/Subst.lean
@@ -1,0 +1,118 @@
+import Mathlib.Data.Fin.Basic
+import CC.Basic
+import CC.Rename
+import CC.CaptureSet
+import CC.Type
+import CC.Context
+import CC.TypeMap
+import CC.Subst
+import CC.Typed
+import CC.Typed.Basic
+import CC.Typed.Rename
+import CC.Subtype
+import CC.Subtype.Subst
+
+namespace CC
+
+theorem Typed.precise_var' (h : Typed Γ t Cx T) :
+  t = Term.var x ->
+  T = CType.capt C S ->
+  Typed Γ t Cx (CType.capt {x} S) := by
+  intro heq1 heq2
+  induction h <;> try (solve | cases heq1 | cases heq2)
+  case var =>
+    cases heq1; cases heq2
+    constructor; trivial
+  case sub =>
+    rename_i hsub ih
+    subst_vars
+    rename_i T0 _
+    cases T0
+    have ih' := ih rfl rfl
+    apply Typed.sub
+    apply ih'
+    constructor
+    apply Subcapt.refl
+    cases hsub; assumption
+
+def Typed.subst {Γ : Ctx n1 m} (h : Typed Γ t C T)
+  {Δ : Ctx n2 m}
+  (σ : VarSubst Γ Δ f) (δ : TVarRename Γ Δ f id) :
+  Typed Δ (t.rename f id) (C.rename f) (T.rename f id) := by
+  induction h generalizing n2
+  case var hb =>
+    have h' := σ hb
+    simp [Term.rename] at *
+    apply Typed.precise_var' <;> try rfl
+    exact h'
+  case sub hsub ih => 
+    apply Typed.sub
+    apply ih <;> trivial
+    apply Subtype.subst hsub <;> aesop
+  case abs ih =>
+    simp [Term.rename]
+    apply Typed.abs
+    apply ih
+    apply VarSubst.ext_var; trivial
+    apply TVarRename.ext_var; trivial
+    apply DropBinder.rename; trivial
+  case tabs ih =>
+    simp [Term.rename]
+    apply Typed.tabs
+    apply ih
+    apply VarSubst.ext_tvar; trivial
+    rw [<- id_ext]
+    apply TVarRename.ext_tvar; trivial
+  case app ih1 ih2 =>
+    simp [Term.rename]
+    simp [CType.rename_open_comm, CaptureSet.rename_union]
+    have ih1' := ih1 σ δ
+    have ih2' := ih2 σ δ
+    apply Typed.app
+    simp [Term.rename] at ih1' ih2'
+    apply ih1'
+    apply ih2'
+  case tapp ih =>
+    simp [Term.rename]
+    simp [CType.rename_open_tvar_comm]
+    have ih' := ih σ δ
+    apply Typed.tapp
+    simp [Term.rename] at ih'
+    apply ih'
+  case box ih =>
+    simp [Term.rename]
+    simp [CType.rename_open_comm, CaptureSet.rename_union]
+    have ih' := ih σ δ
+    apply Typed.box
+    simp [Term.rename] at ih'
+    apply ih'
+  case unbox ih =>
+    simp [Term.rename]
+    simp [CType.rename_open_comm, CaptureSet.rename_union]
+    have ih' := ih σ δ
+    apply Typed.unbox
+    simp [Term.rename] at ih'
+    apply ih'
+  case letval1 ih1 ih2 => 
+    simp [Term.rename]
+    simp [CaptureSet.rename_union]
+    apply Typed.letval1
+    apply ih1 <;> trivial
+    apply ih2
+    apply VarSubst.ext_var; trivial
+    apply TVarRename.ext_var; trivial
+    subst_vars
+    simp [CType.rename_weaken_comm]
+    apply DropBinder.rename; trivial
+  case letval2 ih1 ih2 =>
+    simp [Term.rename]
+    simp [CaptureSet.rename_union]
+    apply Typed.letval2
+    apply ih1 <;> trivial
+    apply Value.rename; trivial
+    apply ih2
+    apply VarSubst.ext_var; trivial
+    apply TVarRename.ext_var; trivial
+    subst_vars
+    simp [CType.rename_weaken_comm]
+    apply DropBinderFree.rename; trivial
